theories/rust_typing/struct/subtype.v
@@ -8,64 +8,116 @@ Section subtype.
   Context `{!typeGS Σ}.
 
   Import EqNotations.
-  Definition struct_t_incl_precond {rts1 rts2 : list RT} (tys1 : hlist type rts1) (tys2 : hlist type rts2) (rs1 : plist place_rfnRT rts1) (rs2 : plist place_rfnRT rts2) :=
+
+  (** Owned subtyping precondition *)
+  Definition struct_t_incl_precond {rts1 rts2 : list RT} π (pers : bool) (tys1 : hlist type rts1) (tys2 : hlist type rts2) (rs1 : plist place_rfnRT rts1) (rs2 : plist place_rfnRT rts2) :=
+    ([∗ list] t1; t2 ∈ hpzipl _ tys1 rs1; hpzipl _ tys2 rs2,
+      match (projT2 t1).2, (projT2 t2).2 with
+      | #r1, #r2 =>
+            ⌜ty_syn_type (projT2 t1).1 MetaNone = ty_syn_type (projT2 t2).1 MetaNone⌝ ∗
+            □?pers owned_type_incl π r1 r2 (projT2 t1).1 (projT2 t2).1
+      | _, _ => ∃ (Heq : projT1 t1 = projT1 t2),
+            ⌜ty_syn_type (projT2 t1).1 MetaNone = ty_syn_type (projT2 t2).1 MetaNone⌝ ∗
+            ⌜(projT2 t1).2 = rew <- [place_rfnRT] Heq in (projT2 t2).2⌝ ∗
+            □?pers ∀ (r : (projT1 t1 : RT)), owned_type_incl π r (rew [RT_rt] Heq in r) (projT2 t1).1 (projT2 t2).1
+      end)%I.
+  Global Instance struct_t_incl_precond_pers π {rts1 rts2} (tys1 : hlist type rts1) (tys2 : hlist type rts2) rs1 rs2 :
+    Persistent (struct_t_incl_precond π true tys1 tys2 rs1 rs2).
+  Proof.
+    apply big_sepL2_persistent. intros ? [? [? []]] [? [? []]]; simpl; apply _.
+  Qed.
+
+  (** Stronger version that also works for sharing *)
+  Definition struct_t_incl_precond_strong {rts1 rts2 : list RT} (tys1 : hlist type rts1) (tys2 : hlist type rts2) (rs1 : plist place_rfnRT rts1) (rs2 : plist place_rfnRT rts2) :=
     ([∗ list] t1; t2 ∈ hpzipl _ tys1 rs1; hpzipl _ tys2 rs2,
       match (projT2 t1).2, (projT2 t2).2 with
       | #r1, #r2 => type_incl r1 r2 (projT2 t1).1 (projT2 t2).1
       | _, _ => ∃ (Heq : projT1 t1 = projT1 t2), ⌜(projT2 t1).2 = rew <- [place_rfnRT] Heq in (projT2 t2).2⌝ ∗ ∀ (r : (projT1 t1 : RT)), type_incl r (rew [RT_rt] Heq in r) (projT2 t1).1 (projT2 t2).1
       end)%I.
-  Global Instance struct_t_incl_precond_pers {rts1 rts2} (tys1 : hlist type rts1) (tys2 : hlist type rts2) rs1 rs2 :
-    Persistent (struct_t_incl_precond tys1 tys2 rs1 rs2).
+  Global Instance struct_t_incl_precond_strong_pers {rts1 rts2} (tys1 : hlist type rts1) (tys2 : hlist type rts2) rs1 rs2 :
+    Persistent (struct_t_incl_precond_strong tys1 tys2 rs1 rs2).
   Proof.
     apply big_sepL2_persistent. intros ? [? [? []]] [? [? []]]; simpl; apply _.
   Qed.
 
-  Lemma struct_t_own_val_mono {rts1 rts2} (tys1 : hlist type rts1) (tys2 : hlist type rts2) rs1 rs2 sls v π m :
-    struct_t_incl_precond tys1 tys2 rs1 rs2 -∗
+  Lemma struct_t_incl_precond_from_strong π {rts1 rts2 : list RT} (tys1 : hlist type rts1) (tys2 : hlist type rts2) (rs1 : plist place_rfnRT rts1) (rs2 : plist place_rfnRT rts2) :
+    struct_t_incl_precond_strong tys1 tys2 rs1 rs2 -∗
+    struct_t_incl_precond π true tys1 tys2 rs1 rs2.
+  Proof.
+    iIntros "Ha". iApply (big_sepL2_impl with "Ha").
+    iModIntro. iIntros (? [rt1 [ty1 r1]] [rt2 [ty2 r2]] Hlook1 Hlook2).
+    simpl.
+    destruct r1 as [r1 | ], r2 as [r2 | ].
+    - iIntros "#Hincl". iSplit; last iApply (type_incl_owned_type_incl with "Hincl").
+      iDestruct "Hincl" as "(% & _)". done.
+    - iIntros "(%Heq & %Ha & _)". destruct Heq. done.
+    - iIntros "(%Heq & %Ha & _)". destruct Heq. done.
+    - iIntros "(%Heq & %Ha & #Hb)". destruct Heq. simpl in *.
+      injection Ha as <-. iExists eq_refl.
+      iSplit. { iDestruct ("Hb" $! inhabitant) as "(%Hst & _)". done. }
+      iR.
+      iIntros (r). iPoseProof (type_incl_owned_type_incl with "Hb") as "Ha"; done.
+  Qed.
+
+  Lemma struct_t_own_val_mono {rts1 rts2} π pers (tys1 : hlist type rts1) (tys2 : hlist type rts2) rs1 rs2 sls v m :
+    struct_t_incl_precond π pers tys1 tys2 rs1 rs2 -∗
     v ◁ᵥ{π, m} rs1 @ struct_t sls tys1 -∗
     v ◁ᵥ{π, m} rs2 @ struct_t sls tys2.
   Proof.
-    iIntros "#Hincl Hv".
+    iIntros "Hincl Hv".
     iPoseProof (big_sepL2_length with "Hincl") as "%Hlen".
     rewrite !length_hpzipl in Hlen.
     iDestruct "Hv" as "(%sl & -> & %Halg & %Hlen1 & %Hly & Hb)".
     iExists sl. iR. rewrite -Hlen. iR. iR. iR.
-    iApply (big_sepL2_impl' with "Hb").
-    { done. }
-    { rewrite !pad_struct_length //. }
-    iModIntro. iIntros (k v1 [rt1 [ty1 r1]] v2 [rt2 [ty2 r2]] Hlook_v1 Hlook_ty1 Hlook_v2 Hlook_ty2) "Hv".
-    iDestruct "Hv" as "(%r' & %ly & Hrfn & %Hly' & %Hst' & Hv)".
-    rewrite Hlook_v2 in Hlook_v1. injection Hlook_v1 as ->.
-    apply pad_struct_lookup_Some in Hlook_ty1 as (n & ly' & Hly'' & Hlook_ty1).
-    2: { rewrite length_hpzipl Hlen1. symmetry. by apply struct_layout_spec_has_layout_fields_length. }
-    rewrite Hly'' in Hly'. injection Hly' as ->.
-    eapply pad_struct_lookup_Some_1' in Hlook_ty2; last done; first last.
-    { rewrite length_hpzipl -Hlen Hlen1. symmetry. by apply struct_layout_spec_has_layout_fields_length. }
-    destruct Hlook_ty1 as [ [? Hlook_ty1] | (-> & Hlook_ty1)]; first last.
-    { (* padding *)
-      destruct Hlook_ty2 as [ [? ?] | [_ Hlook_ty2]]; first congruence.
-      injection Hlook_ty1 => _ _ ?; subst.
-      injection Hlook_ty2 => _ _ ?; subst.
-      apply existT_inj in Hlook_ty1. injection Hlook_ty1 as -> ->.
-      apply existT_inj in Hlook_ty2. injection Hlook_ty2 as -> ->.
-      iExists r', ly. rewrite Hly''. iFrame. done. }
-    (* element *)
-    destruct Hlook_ty2 as [[_ Hlook_ty2] | [? _]]; last congruence.
-    rewrite /struct_own_el_val.
-    iPoseProof (big_sepL2_lookup with "Hincl") as "Ha"; [apply Hlook_ty1 | apply Hlook_ty2 | ]; simpl.
-    destruct r1 as [r1 | ]; first destruct r2 as [r2 | ].
-    + iDestruct "Hrfn" as "<-".
-      iDestruct "Ha" as "(%Hst & _ & #Ha & _)". iPoseProof ("Ha" with "Hv") as "Hv".
-      rewrite Hly'' -Hst. eauto with iFrame.
-    + iDestruct "Ha" as "(%Heq & %Heq' & Ha)". subst.
-      iDestruct "Hrfn" as "<-". done.
-    + iDestruct "Ha" as "(%Heq & %Heq' & Ha)". subst. cbn in Heq'. subst.
-      iDestruct ("Ha" $! r') as "(%Hst & _ & #Ha' & _)". iPoseProof ("Ha'" with "Hv") as "Hv".
-      rewrite Hly'' -Hst. eauto with iFrame.
+
+    iApply big_sepL2_from_big_sepL_lookup_l.
+    { rewrite pad_struct_length length_reshape !length_fmap//. }
+    iPoseProof (big_sepL2_to_big_sepL_lookup_l with "Hb") as "Hb".
+    iApply big_sepL2_elim_l.
+    iPoseProof (big_sepL_extend_r with "Hb") as "Hb"; last (iApply (big_sepL2_wand with "Hb")).
+    { rewrite !pad_struct_length//. }
+
+    opose proof (struct_layout_spec_has_layout_fields_length _ _ Halg) as Hlen'.
+    iApply (pad_struct_unfocus_big_sepL2 with "[Hincl]").
+    { rewrite length_hpzipl named_fields_field_names_length.
+      erewrite struct_layout_spec_has_layout_fields_length; done. }
+    { rewrite length_hpzipl named_fields_field_names_length.
+      rewrite -Hlen Hlen'. done. }
+    { apply field_names_NoDup. }
+    { iApply (big_sepL2_impl with "Hincl").
+      iModIntro. iIntros (k [rt1 [ty1 r1]] [rt2 [ty2 r2]] Hlook1 Hlook2). simpl.
+      iIntros "Hincl".
+      specialize (hpzipl_lookup_inv rts1 _ _ _ _ _ _ Hlook1) as Hlook1'.
+      specialize (hpzipl_lookup_inv _ _ _ _ _ _ _ Hlook2) as Hlook2'.
+      apply lookup_lt_Some in Hlook1'. apply lookup_lt_Some in Hlook2'.
+      opose proof (lookup_lt_is_Some_2 (named_fields (sl_members sl)) k _) as ([x ly] & Hfield).
+      { rewrite named_fields_field_names_length. lia. }
+      opose proof (named_fields_lookup_1 _ _ _ _ Hfield) as (j & Hfield').
+      iExists _, ly, x. iR. iR.
+      iIntros "(%v' & %Hv & %r' & %ly' & Hrfn & % & %Hst1 & Hown)".
+      iExists v'. iR.
+      destruct r1 as [r1 | ]; first destruct r2 as [r2 | ].
+      + iDestruct "Hrfn" as "<-".
+        iDestruct "Hincl" as "(%Hst_eq & Hincl)".
+        iPoseProof (bi.intuitionistically_if_elim with "Hincl") as "(%Hst & Hsc & Hincl)".
+        iPoseProof ("Hincl" with "Hown") as "Hown".
+        rewrite Hst_eq in Hst1.
+        iExists r2, ly'. iR. iR. iR. done.
+      + iDestruct "Hincl" as "(%Heq & %Hst & %Heq' & Ha)". subst.
+        done.
+      + iDestruct "Hincl" as "(%Heq & %Hst & %Heq' & Hincl)". subst.
+        iPoseProof (bi.intuitionistically_if_elim with "Hincl") as "Ha".
+        cbn in Heq'. subst.
+        iDestruct ("Ha" $! r') as "(_ & _ & Ha)". iPoseProof ("Ha" with "Hown") as "Hv".
+        iExists r', _. iFrame. iR. rewrite -Hst. done. }
+    { simpl. iApply big_sepL_intro.
+      iModIntro. iIntros (? [ly | ] Hlook); last done.
+      simpl. eauto. }
   Qed.
 
+
   Lemma struct_t_shr_mono {rts1 rts2} (tys1 : hlist type rts1) (tys2 : hlist type rts2) rs1 rs2 sls l κ π m :
-    struct_t_incl_precond tys1 tys2 rs1 rs2 -∗
+    struct_t_incl_precond_strong tys1 tys2 rs1 rs2 -∗
     l ◁ₗ{π, m, κ} rs1 @ struct_t sls tys1 -∗
     l ◁ₗ{π, m, κ} rs2 @ struct_t sls tys2.
   Proof.
@@ -110,7 +162,7 @@ Section subtype.
   Qed.
 
   Lemma struct_t_type_incl {rts1 rts2} (tys1 : hlist type rts1) (tys2 : hlist type rts2) rs1 rs2 sls :
-    struct_t_incl_precond tys1 tys2 rs1 rs2 -∗
+    struct_t_incl_precond_strong tys1 tys2 rs1 rs2 -∗
     type_incl rs1 rs2 (struct_t sls tys1) (struct_t sls tys2).
   Proof.
     iIntros "#Hincl".
@@ -118,7 +170,8 @@ Section subtype.
     rewrite !length_hpzipl in Hlen.
     iSplitR; first done. iSplitR. { simpl. rewrite Hlen. done. }
     iSplit; iModIntro.
-    - iIntros (???). by iApply struct_t_own_val_mono.
+    - iIntros (???). iApply struct_t_own_val_mono.
+      by iApply struct_t_incl_precond_from_strong.
     - iIntros (????). by iApply struct_t_shr_mono.
   Qed.
 
